theories/RecSig.v
@@ -1,0 +1,14 @@
+From Coq Require Import String.
+From Hammer Require Import Tactics.
+From LambdaST Require Import
+  Context
+  Hole
+  Sets
+  Subcontext
+  Inert
+  Types.
+
+Inductive recsig : Set :=
+  | NoRec : recsig
+  | Rec : context -> type -> inertness -> recsig.
+Hint Constructors recsig : core.
